[StateLib Crdt examples] pn counter implementation, fixed gcounter implementation and proof.

ml_sources/examples/crdt/statelib/examples/gcounter/gcounter_code.ml
@@ -1,0 +1,39 @@
+open !Ast
+open List_code
+open Vector_clock_code
+open Statelib_code
+
+(* TODO : move to List_code *)
+let rec list_map2 (f : 'a -> 'b -> 'c) (l : 'a alist) (l' : 'b alist) : 'c alist =
+  match l with
+    Some a ->
+    begin
+      match l' with
+      | Some b ->
+        list_cons (f (fst a) (fst b)) (list_map2 f (snd a) (snd b))
+      | None -> assert false
+    end
+  | None -> None
+
+let gcpt_init_st n = fun () -> vect_make n 0
+
+let gcpt_mutator : (int, int alist) mutatorFnTy =
+  fun (repId : int) (st : int alist) (op : int) ->
+  match list_nth st repId with
+  | None -> st
+  | Some p -> vect_update st repId (op + p)
+
+let max_fn i j = if i < j then j else i
+
+let gcpt_merge st st' :'a alist = list_map2 max_fn st st'
+
+let gcpt_crdt n : (int, int alist) crdtTy =
+  fun () -> (((fun () -> gcpt_init_st n ()), gcpt_mutator), gcpt_merge)
+
+let gcpt_init addrs rid =
+  let len = list_length addrs in
+  let initRes =
+    statelib_init vect_serialize vect_deserialize addrs rid (gcpt_crdt len) in
+  let get_state = fst initRes in
+  let update = snd initRes in
+  (get_state, update)
