ml_sources/examples/crdt/statelib/examples/grow_only_set/grow_only_set_code.ml
@@ -6,16 +6,17 @@ open Statelib_code
 
 type 'a stTy = 'a aset
 
-let mutator : ('a, 'stTy) mutatorFnTy =
+let gos_init_st () = set_empty ()
+
+let gos_mutator : ('a, 'stTy) mutatorFnTy =
   fun (_i : int) (gs : 'stTy) (op : 'a) ->
   set_add op gs
 
-let merge (st1 : 'a stTy) (st2 : 'a stTy) : 'a stTy =
+let gos_merge (st1 : 'a stTy) (st2 : 'a stTy) : 'a stTy =
   set_union st1 st2
 
-let init_st () = set_empty ()
-
-let gos_crdt : ('a, 'a stTy) crdtTy = fun () -> ((init_st, mutator), merge)
+let gos_crdt : ('a, 'a stTy) crdtTy =
+  fun () -> ((gos_init_st, gos_mutator), gos_merge)
 
 let gos_init  (elt_ser[@metavar "val"]) (elt_deser[@metavar "val"])
     (addrs : saddr alist) (rid : int) =
