ml_sources/examples/crdt/statelib/examples/pncounter/pncounter_code.ml
@@ -1,0 +1,64 @@
+open !Ast
+open Serialization_code
+open List_code
+open Vector_clock_code
+open Statelib_code
+open Gcounter_code
+open Prod_comb_code
+
+(** Step 1. Raw PN counter using product and gcpt crdts. *)
+
+type pnCptStTy = (int alist, int alist) stProdTy
+type pnCptOpTy = (int, int) opProdTy
+
+let pn_cpt_init_st n : unit -> pnCptStTy =
+  fun () -> prod_init_st (gcpt_init_st n) (gcpt_init_st n) ()
+
+let pn_cpt_mutator : (pnCptOpTy, pnCptStTy) mutatorFnTy =
+  fun (i : int) (cpt : pnCptStTy) (op : pnCptOpTy) ->
+  let (p, n) = op in
+  assert ((0 = p && 0 = n) || (p < 0 && n = 0) || (n < 0 && p = 0));
+  prod_mutator gcpt_mutator gcpt_mutator i cpt op
+
+let pn_cpt_merge (st : pnCptStTy) (st' : pnCptStTy) : pnCptStTy =
+  prod_merge gcpt_merge gcpt_merge st st'
+
+
+let pn_cpt_crdt n : (pnCptOpTy, pnCptStTy) crdtTy =
+  fun () -> ((pn_cpt_init_st n, pn_cpt_mutator), pn_cpt_merge)
+
+let pn_cpt_init addrs rid =
+  let len = list_length addrs in
+  let initRes =
+    statelib_init
+      (prod_ser vect_serialize vect_serialize)
+      (prod_deser vect_deserialize vect_deserialize)
+      addrs rid (pn_cpt_crdt len) in
+  let get_state = fst initRes in
+  let update = snd initRes in
+  (get_state, update)
+
+(** Step 2. PN counter wrapper. *)
+
+(* TODO : move to List_code *)
+let list_int_sum (l : int alist) =
+  list_fold (fun acc n -> acc + n) 0 l
+
+let pncounter_update (upd : pnCptOpTy -> unit) (n : int) =
+  if 0 <= n
+  then upd (n, 0)
+  else upd (0, n)
+
+let pncounter_eval (get_state : unit -> pnCptStTy) () =
+  let st = get_state () in
+  let (pl, nl) = st in
+  let p = list_int_sum pl in
+  let n = list_int_sum nl in
+  p + n
+
+let pncounter_init addrs rid =
+  let pn_cpt = pn_cpt_init addrs rid in
+  let (get_st, upd_st) = pn_cpt in
+  let get = pncounter_eval get_st in
+  let upd = pncounter_update upd_st in
+  (get, upd)
