ml_sources/examples/crdt/statelib/examples/prod_comb/prod_comb_code.ml
@@ -23,7 +23,10 @@ type  ('opA, 'opB, 'stA, 'stB) crdtProdTy =
  *     ('opA, 'opB, 'stA, 'stB) mutatorProdFnTy) *
  *     ('stA, 'stB) mergeProdFnTy) *)
 
-let mutator
+let prod_init_st init_fnA init_fnB : ('stA, 'stB) init_stProdFnTy =
+  fun () -> (init_fnA (), init_fnB ())
+
+let prod_mutator
     (mut_fnA : ('opA, 'stA) mutatorFnTy)
     (mut_fnB : ('opB, 'stB) mutatorFnTy)
   : ('opA, 'opB, 'stA, 'stB) mutatorProdFnTy =
@@ -32,7 +35,7 @@ let mutator
   let (opA, opB) = op in
   (mut_fnA i gsA opA, mut_fnB i gsB opB)
 
-let merge
+let prod_merge
     (merge_fnA : 'stA mergeFnTy)
     (merge_fnB : 'stB mergeFnTy)
   : ('stA, 'stB) mergeProdFnTy =
@@ -43,12 +46,9 @@ let merge
    let mB = merge_fnB st12 st22 in
    (mA, mB)
 
-let init_st init_fnA init_fnB : ('stA, 'stB) init_stProdFnTy =
-  fun () -> (init_fnA (), init_fnB ())
-
 let prod_crdt
-  (cA : ('opA, 'stA) crdtTy)
-  (cB : ('opB, 'stB) crdtTy)
+  (cA[@metavar "val"] : ('opA, 'stA) crdtTy)
+  (cB[@metavar "val"] : ('opB, 'stB) crdtTy)
   :  (('opA, 'opB) opProdTy, ('stA, 'stB) stProdTy) crdtTy =
   (* :  ('opA, 'opB, 'stA, 'stB) crdtProdTy = *)
   fun () ->
@@ -56,21 +56,21 @@ let prod_crdt
   let cBp = cB () in
   let ((init_fnA, mut_fnA), merge_fnA) = cAp in
   let ((init_fnB, mut_fnB), merge_fnB) = cBp in
-  let init_fn = init_st init_fnA init_fnB in
-  let mut_fn = mutator mut_fnA mut_fnB in
-  let merge_fn = merge merge_fnA merge_fnB in
+  let init_fn = (fun () -> prod_init_st init_fnA init_fnB ()) in
+  let mut_fn = (fun i gs op -> prod_mutator mut_fnA mut_fnB i gs op) in
+  let merge_fn = (fun st1 st2 -> prod_merge merge_fnA merge_fnB st1 st2) in
   ((init_fn, mut_fn), merge_fn)
 
 let prod_init
     (stA_ser[@metavar "val"]) (stA_deser[@metavar "val"])
     (stB_ser[@metavar "val"]) (stB_deser[@metavar "val"])
-    (cA : ('opA, 'stA) crdtTy)
-    (cB : ('opB, 'stB) crdtTy)
+    (cA[@metavar "val"] : ('opA, 'stA) crdtTy)
+    (cB[@metavar "val"] : ('opB, 'stB) crdtTy)
     (addrs : saddr alist) (rid : int) =
   let initRes =
     statelib_init
       (prod_ser stA_ser stB_ser)
       (prod_deser stA_deser stB_deser)
-      addrs rid (prod_crdt cA cB) in
+      addrs rid (fun () -> prod_crdt cA cB ()) in
   let (get_state, update) = initRes in
   (get_state, update)
